theories/SetModel/HO_prop.v
@@ -15,12 +15,6 @@ Proof.
     + apply empty_in_univ.
 Qed.
 
-Lemma propTy_HO_typing' {n : nat} {Γ : ZFSet} : ∀ γ ∈ Γ, propTy_HO γ ∈ 𝕌el (S n) (univTy_HO n γ).
-Proof.
-  intros γ Hγ. refine (transpS (fun X => _ ∈ X) (sym _) (propTy_HO_typing γ Hγ)).
-  now apply el_univTy.
-Qed.
-
 Lemma el_propTy {n : nat} {γ : ZFSet} : 𝕌el n (propTy_HO γ) ≡ Ω.
 Proof.
   apply setPairβ1.
