theories/SetModel/model_obseq.v
@@ -10,24 +10,140 @@ Require Import ZF_axioms ZF_library ZF_nat ZF_acc.
 Require Import HO HO_univ HO_prop HO_box HO_pi HO_sigma HO_nat HO_acc HO_obseq HO_forall.
 Require Import model_interp model_def.
 
-Lemma model_obseq (Γ : ctx) (i : level) (A a b : term) (tA : Γ ⊢< Ax i > A : Sort i) (mA : model_typing Γ (Ax i) A (Sort i))
-  (ta : Γ ⊢< i > a : A) (ma : model_typing Γ i a A)
-  (tb : Γ ⊢< i > b : A) (mb : model_typing Γ i b A) :
-  model_typing Γ (Ax prop) (obseq i A a b) (Sort prop).
+Lemma model_obseq (Γ : ctx) (i : nat) (A a b : term)
+  (tA : Γ ⊢< Ax (ty i) > A : Sort (ty i)) (mA : model_typing Γ (Ax (ty i)) A (Sort (ty i)))
+  (ta : Γ ⊢< ty i > a : A) (ma : model_typing Γ (ty i) a A)
+  (tb : Γ ⊢< ty i > b : A) (mb : model_typing Γ (ty i) b A) :
+  model_typing Γ (Ax prop) (obseq (ty i) A a b) (Sort prop).
+Proof.
+  apply to_model_prop.
+  destruct ma as [ iΓ fΓ iA fA ia fa vA va ]. destruct mb as [ iΓ' fΓ' iA' fA' ib fb vA' vb ].
+  destruct (functional_ctx Γ fΓ fΓ'). destruct (functional_tm A fA fA'). clear fΓ' fA' vA'. econstructor.
+  + exact fΓ.
+  + apply interp_obseq_r. exact fA. exact fa. exact fb.
+  + eapply eqTy_HO_typing. exact vA. exact va. exact vb.
+Qed.
+
+Lemma model_obsrefl (l : nat) (Γ : ctx) (A a : term)
+  (tA : Γ ⊢< Ax (ty l) > A : Sort (ty l)) (mA : model_typing Γ (Ax (ty l)) A (Sort (ty l)))
+  (ta : Γ ⊢< ty l > a : A) (ma : model_typing Γ (ty l) a A) :
+  model_typing Γ prop (obsrefl (ty l) A a) (obseq (ty l) A a a).
+Proof.
+  destruct ma as [ iΓ fΓ iA fA ia fa vA va ]. econstructor.
+  - exact fΓ.
+  - apply interp_obseq_r. exact fA. exact fa. exact fa.
+  - eapply eqTy_HO_typing. exact vA. exact va. exact va.
+  - eapply reflTm_HO_typing. exact vA. exact va.
+Qed.
+
+Lemma model_J (Γ : ctx) (l : nat) (A a P p b e : term)
+  (tA : Γ ⊢< Ax (ty l) > A : Sort (ty l)) (mA : model_typing Γ (Ax (ty l)) A (Sort (ty l)))
+  (ta : Γ ⊢< ty l > a : A) (ma : model_typing Γ (ty l) a A)
+  (tP : Γ,, (ty l, A) ⊢< Ax prop > P : Sort prop) (mP : model_typing (Γ,, (ty l, A)) (Ax prop) P (Sort prop))
+  (tp : Γ ⊢< prop > p : P <[ a..]) (mp : model_typing Γ prop p (P <[ a..]))
+  (tb : Γ ⊢< ty l > b : A) (mb : model_typing Γ (ty l) b A)
+  (te : Γ ⊢< prop > e : obseq (ty l) A a b) (me : model_typing Γ prop e (obseq (ty l) A a b)) :
+  model_typing Γ prop (J (ty l) A a P p b e) (P <[ b..]).
+Proof.
+Admitted.
+
+Lemma model_cast (Γ : ctx) (i : level) (A B e a : term)
+  (tA : Γ ⊢< Ax i > A : Sort i) (mA : model_typing Γ (Ax i) A (Sort i))
+  (tB : Γ ⊢< Ax i > B : Sort i) (mB : model_typing Γ (Ax i) B (Sort i))
+  (te : Γ ⊢< prop > e : obseq (Ax i) (Sort i) A B) (me : model_typing Γ prop e (obseq (Ax i) (Sort i) A B))
+  (ta : Γ ⊢< i > a : A) (ma : model_typing Γ i a A) :
+  model_typing Γ i (cast i A B e a) B.
 Proof.
   destruct i as [ i | ].
-  - destruct ma as [ iΓ fΓ iA fA ia fa vA va ]. destruct mb as [ iΓ' fΓ' iA' fA' ib fb vA' vb ].
-    destruct (functional_ctx Γ fΓ fΓ'). destruct (functional_tm A fA fA'). clear fΓ' fA' vA'. econstructor.
+  (* Proof-relevant cast *)
+  - destruct ma as [ iΓ fΓ iA fA ia fa vA va ]. apply of_model_univ in mB. destruct mB as [ iΓ' fΓ' iB fB vB ].
+    destruct (functional_ctx Γ fΓ fΓ'). clear fΓ'.
+    destruct me as [ iΓ' fΓ' iE fE vE ve ]. destruct (functional_ctx Γ fΓ fΓ'). clear fΓ'.
+    inversion fE ; subst ; clear fE.
+    inversion H4 ; subst ; clear H4.
+    destruct (functional_tm A fA H6). clear H6. destruct (functional_tm B fB H7). clear H7. 
+    econstructor.
     + exact fΓ.
-    + apply interp_prop.
-    + apply interp_obseq_r. exact fA. exact fa. exact fb.
-    + apply propTy_HO_typing.
-    + eapply eqTy_HO_typing'. exact vA. exact va. exact vb.
-  - destruct ma as [ iΓ fΓ iA fA vA va ]. destruct mb as [ iΓ' fΓ' iA' fA' vA' vb ].
-    destruct (functional_ctx Γ fΓ fΓ'). destruct (functional_tm A fA fA'). clear fΓ' fA' vA'. econstructor.
+    + exact fB.
+    + apply interp_cast. exact fA. exact fB. exact fa.
+    + exact vB.
+    + eapply castTm_HO_typing. exact vA. exact ve. exact va.
+  (* Proof-irrelevant cast *)
+  - destruct ma as [ iΓ fΓ iA fA vA va ]. apply of_model_univ in mB. destruct mB as [ iΓ' fΓ' iB fB vB ].
+    destruct (functional_ctx Γ fΓ fΓ'). clear fΓ'.
+    destruct me as [ iΓ' fΓ' iE fE vE ve ]. destruct (functional_ctx Γ fΓ fΓ'). clear fΓ'.
+    inversion fE ; subst ; clear fE.
+    inversion H4 ; subst ; clear H4.
+    destruct (functional_tm A fA H6). clear H6. destruct (functional_tm B fB H7). clear H7. 
+    econstructor.
     + exact fΓ.
-    + apply interp_prop.
-    + apply interp_obseq_i. 
-    + apply propTy_HO_typing.
-    + intros. refine (transpS (fun X => ⋆ ∈ X) (sym _) _). apply el_propTy. now apply ZFinpower. 
+    + exact fB.
+    + exact vB.
+    + intros γ Hγ. specialize (ve γ Hγ). apply subsingl_true_if in ve.
+      exact (transpS (fun X => ∅ ∈ X) ve (va γ Hγ)).
 Qed.
+
+Lemma model_injpi1 (Γ : ctx) (i : level) (j : nat) (A1 A2 B1 B2 e : term)
+  (tA1 : Γ ⊢< Ax i > A1 : Sort i) (mA1 : model_typing Γ (Ax i) A1 (Sort i))
+  (tB1 : Γ,, (i, A1) ⊢< Ax (ty j) > B1 : Sort (ty j)) (mB1 : model_typing (Γ,, (i, A1)) (Ax (ty j)) B1 (Sort (ty j)))
+  (tA2 : Γ ⊢< Ax i > A2 : Sort i) (mA2 : model_typing Γ (Ax i) A2 (Sort i))
+  (tB2 : Γ,, (i, A2) ⊢< Ax (ty j) > B2 : Sort (ty j)) (mB2 : model_typing (Γ,, (i, A2)) (Ax (ty j)) B2 (Sort (ty j)))
+  (te : Γ ⊢< prop > e : obseq (Ax (Ru i (ty j))) (Sort (Ru i (ty j))) (Pi i (ty j) A1 B1) (Pi i (ty j) A2 B2))
+  (me : model_typing Γ prop e (obseq (Ax (Ru i (ty j))) (Sort (Ru i (ty j))) (Pi i (ty j) A1 B1) (Pi i (ty j) A2 B2))) :
+  model_typing Γ prop (injpi1 i (ty j) A1 A2 B1 B2 e) (obseq (Ax i) (Sort i) A2 A1).
+Proof.
+  apply of_model_univ in mA1. apply of_model_univ in mA2. apply of_model_univ in mB1. apply of_model_univ in mB2.
+  destruct i as [ i | ].
+  (* relevant domain *)
+  - destruct mA1 as [ iΓ fΓ iA1 fA1 vA1 ]. destruct mA2 as [ iΓ' fΓ' iA2 fA2 vA2 ].
+    destruct (functional_ctx Γ fΓ fΓ') ; clear fΓ'. destruct mB1 as [ iΓ' fΓ' iB1 fB1 vB1 ].
+    inversion fΓ' ; subst ; clear fΓ'. destruct (functional_ctx Γ fΓ H3) ; clear H3.
+    destruct (functional_tm A1 fA1 H4) ; clear H4. destruct mB2 as [ iΓ' fΓ' iB2 fB2 vB2 ].
+    inversion fΓ' ; subst ; clear fΓ'. destruct (functional_ctx Γ fΓ H3) ; clear H3.
+    destruct (functional_tm A2 fA2 H4) ; clear H4. destruct me as [ iΓ' fΓ' iE fE vE ve ].
+    destruct (functional_ctx Γ fΓ fΓ') ; clear fΓ'. inversion fE ; subst ; clear fE.
+    inversion H4 ; subst ; clear H4. inversion H6 ; subst ; clear H6. destruct (functional_tm A1 fA1 H8) ; clear H8.
+    destruct (functional_tm B1 fB1 H9) ; clear H9. clear H. inversion H7 ; subst ; clear H7.
+    destruct (functional_tm A2 fA2 H6) ; clear H6. destruct (functional_tm B2 fB2 H8) ; clear H8. clear H.
+    econstructor.
+    + exact fΓ.
+    + apply interp_obseq_r. apply interp_type. exact fA2. exact fA1.
+    + eapply eqTy_HO_typing.
+      * apply univTy_HO_typing.
+      * intros γ Hγ. refine (transpS (fun X => _ ∈ X) (sym _) (vA2 γ Hγ)). now apply el_univTy.
+      * intros γ Hγ. refine (transpS (fun X => _ ∈ X) (sym _) (vA1 γ Hγ)). now apply el_univTy.
+    + apply (piinj1Tm_HO_typing vA1 vB1 vA2 vB2 ve).
+  (* irrelevant domain *)
+  - destruct mA1 as [ iΓ fΓ iA1 fA1 vA1 ]. destruct mA2 as [ iΓ' fΓ' iA2 fA2 vA2 ].
+    destruct (functional_ctx Γ fΓ fΓ') ; clear fΓ'. destruct mB1 as [ iΓ' fΓ' iB1 fB1 vB1 ].
+    inversion fΓ' ; subst ; clear fΓ'. destruct (functional_ctx Γ fΓ H1) ; clear H1.
+    destruct (functional_tm A1 fA1 H3) ; clear H3. destruct mB2 as [ iΓ' fΓ' iB2 fB2 vB2 ].
+    inversion fΓ' ; subst ; clear fΓ'. destruct (functional_ctx Γ fΓ H1) ; clear H1.
+    destruct (functional_tm A2 fA2 H3) ; clear H3. destruct me as [ iΓ' fΓ' iE fE vE ve ].
+    destruct (functional_ctx Γ fΓ fΓ') ; clear fΓ'. inversion fE ; subst ; clear fE.
+    inversion H4 ; subst ; clear H4. inversion H6 ; subst ; clear H6. destruct (functional_tm A1 fA1 H3) ; clear H3.
+    destruct (functional_tm B1 fB1 H5) ; clear H5. inversion H7 ; subst ; clear H7.
+    destruct (functional_tm A2 fA2 H3) ; clear H3. destruct (functional_tm B2 fB2 H5) ; clear H5. 
+    econstructor.
+    + exact fΓ.
+    + apply interp_obseq_r. apply interp_prop. exact fA2. exact fA1.
+    + unshelve eapply eqTy_HO_typing.
+      * exact 0.
+      * apply propTy_HO_typing.
+      * intros γ Hγ. refine (transpS (fun X => _ ∈ X) (sym _) (vA2 γ Hγ)). now apply el_propTy.
+      * intros γ Hγ. refine (transpS (fun X => _ ∈ X) (sym _) (vA1 γ Hγ)). now apply el_propTy.
+    + apply (piinj1Tm_HO_typing_ir vA1 vB1 vA2 vB2 ve). 
+Qed.
+
+Lemma model_injpi2 (Γ : ctx) (i : level) (j : nat) (A1 A2 B1 B2 e a2 : term)
+  (tA1 : Γ ⊢< Ax i > A1 : Sort i) (mA1 : model_typing Γ (Ax i) A1 (Sort i))
+  (tB1 : Γ,, (i, A1) ⊢< Ax (ty j) > B1 : Sort (ty j)) (mB1 : model_typing (Γ,, (i, A1)) (Ax (ty j)) B1 (Sort (ty j)))
+  (tA2 : Γ ⊢< Ax i > A2 : Sort i) (mA2 : model_typing Γ (Ax i) A2 (Sort i))
+  (tB2 : Γ,, (i, A2) ⊢< Ax (ty j) > B2 : Sort (ty j)) (mB2 : model_typing (Γ,, (i, A2)) (Ax (ty j)) B2 (Sort (ty j)))
+  (te : Γ ⊢< prop > e : obseq (Ax (Ru i (ty j))) (Sort (Ru i (ty j))) (Pi i (ty j) A1 B1) (Pi i (ty j) A2 B2))
+  (me : model_typing Γ prop e (obseq (Ax (Ru i (ty j))) (Sort (Ru i (ty j))) (Pi i (ty j) A1 B1) (Pi i (ty j) A2 B2)))
+  (ta2 : Γ ⊢< i > a2 : A2) (ma2 : model_typing Γ i a2 A2)
+  (a1 := cast i A2 A1 (injpi1 i (ty j) A1 A2 B1 B2 e) a2) :
+  model_typing Γ prop (injpi2 i (ty j) A1 A2 B1 B2 e a2) (obseq (Ax (ty j)) (Sort (ty j)) (B1 <[ a1..]) (B2 <[ a2..])).
+Proof.
+Admitted.
