theories/SetModel/model_pi.v
@@ -15,48 +15,33 @@ Lemma model_pi (Γ : ctx) (i j : level) (A B : term) (tA : Γ ⊢< Ax i > A : So
   (tB : Γ,, (i, A) ⊢< Ax j > B : Sort j) (mB : model_typing (Γ,, (i, A)) (Ax j) B (Sort j)) :
   model_typing Γ (Ax (Ru i j)) (Pi i j A B) (Sort (Ru i j)).
 Proof.
-  destruct mA as [ iΓ fΓ iS fS iA fA vS vA ]. destruct mB as [ iΓ' fΓ' iT fT iB fB vT vB ].
-  inversion fS ; subst ; clear fS. 
-  all: inversion fΓ' ; subst ; clear fΓ'.
-  1: destruct (functional_ctx Γ fΓ H4) ; clear H4. 2: destruct (functional_ctx Γ fΓ H2) ; clear H2.
-  1: destruct (functional_tm A fA H5) ; clear H5. 2: destruct (functional_tm A fA H4) ; clear H4.
-  all: inversion fT ; subst ; clear fT.
+  apply of_model_univ in mA. apply of_model_univ in mB.
+  destruct i as [ i | ] ; destruct j as [ j | ]. all: destruct mA ; destruct mB.
+  all: inversion fΓ0 ; subst ; clear fΓ0.
+  1,2: destruct (functional_ctx Γ fΓ H3) ; clear H3. 3,4: destruct (functional_ctx Γ fΓ H1) ; clear H1.
+  1,2: destruct (functional_tm A fA H4) ; clear H4. 3,4: destruct (functional_tm A fA H3) ; clear H3.
   (* Pi (relevant relevant) *)
-  + econstructor.
+  + apply to_model_univ. econstructor.
     * exact fΓ.
-    * apply interp_type.
-    * apply interp_pi_rr. exact fA. exact fB.
-    * apply univTy_HO_typing.
-    * apply piTy_HO_typing'.
-      ** intros γ Hγ. refine (transpS (fun X => iA γ ∈ X) _ (vA γ Hγ)). now apply el_univTy.
-      ** intros γa Hγa. refine (transpS (fun X => iB γa ∈ X) _ (vB γa Hγa)). now apply el_univTy.
+    * apply interp_pi_rr. exact fA. exact fA0.
+    * apply piTy_HO_typing. exact vA. exact vA0. 
   (* Pi (relevant irrelevant) *)
-  + inversion H1. subst. econstructor.
+  + apply to_model_univ. econstructor.
     * exact fΓ.
-    * apply interp_prop.
-    * apply interp_pi_ri. exact fA. exact fB.
-    * apply propTy_HO_typing.
-    * apply forallTy_HO_typing'.
-      ** intros γ Hγ. refine (transpS (fun X => iA γ ∈ X) _ (vA γ Hγ)). now apply el_univTy.
-      ** intros γa Hγa. refine (transpS (fun X => iB γa ∈ X) _ (vB γa Hγa)). now apply el_propTy.
+    * apply interp_pi_ri. exact fA. exact fA0.
+    * apply forallTy_HO_typing. exact vA. exact vA0.
   (* Pi (irrelevant relevant) *)
-  + econstructor.
+  + apply to_model_univ. econstructor.
     * exact fΓ.
-    * apply interp_type.
-    * apply interp_pi_ir. exact fA. exact fB.
-    * apply univTy_HO_typing.
-    * apply piTy_HO_typing_ir'.
-      ** intros γ Hγ. refine (transpS (fun X => iA γ ∈ X) _ (vA γ Hγ)). now apply el_propTy.
-      ** intros γa Hγa. refine (transpS (fun X => iB γa ∈ X) _ (vB γa Hγa)). now apply el_univTy.
+    * apply interp_pi_ir. exact fA. exact fA0.
+    * apply piTy_HO_typing_ir. exact vA. exact vA0.
   (* Pi (irrelevant irrelevant) *)
-  + econstructor.
+  + apply to_model_univ. econstructor.
     * exact fΓ.
-    * apply interp_prop.
-    * apply interp_pi_ii. exact fA. exact fB.
-    * apply propTy_HO_typing.
-    * apply forallTy_HO_typing'.
-      ** apply boxTy_HO_typing. intros γ Hγ. refine (transpS (fun X => iA γ ∈ X) _ (vA γ Hγ)). now apply el_propTy.
-      ** intros γa Hγa. refine (transpS (fun X => iB γa ∈ X) _ (vB γa Hγa)). now apply el_propTy.
+    * apply interp_pi_ii. exact fA. exact fA0.
+    * apply forallTy_HO_typing. 
+      ** apply boxTy_HO_typing. exact vA. 
+      ** exact vA0. 
 Qed.
 
 Lemma model_lambda (Γ : ctx) (i j : level) (A B t : term) (tA : Γ ⊢< Ax i > A : Sort i) (mA : model_typing Γ (Ax i) A (Sort i))
@@ -64,61 +49,42 @@ Lemma model_lambda (Γ : ctx) (i j : level) (A B t : term) (tA : Γ ⊢< Ax i > 
   (tt : Γ,, (i, A) ⊢< j > t : B) (mt : model_typing (Γ,, (i, A)) j t B) :
   model_typing Γ (Ru i j) (lam i j A B t) (Pi i j A B).
 Proof.
-  destruct mA as [ iΓ fΓ iS fS iA fA vS vA ]. destruct j as [ j | ].
-  - destruct mt as [ iΓ' fΓ' iB fB it ft vB vt ]. inversion fΓ' ; subst ; clear fΓ'.
-    all: destruct (functional_ctx Γ fΓ H3) ; clear H3. 
-    all: destruct (functional_tm A fA H4) ; clear H4. 
-    all: inversion fS ; subst ; clear fS.
+  apply of_model_univ in mA. destruct j as [ j | ]. 
+  - destruct mt as [ iΓ' fΓ' iB fB it ft vB vt ]. destruct i as [ i | ] ; destruct mA as [ iΓ fΓ iA fA vA ].
+    all: inversion fΓ' ; subst ; clear fΓ'.
     (* lambda (relevant relevant) *)
-    + econstructor.
+    + destruct (functional_ctx Γ fΓ H3) ; clear H3. destruct (functional_tm A fA H4) ; clear H4. econstructor.
       * exact fΓ.
       * apply interp_pi_rr. exact fA. exact fB.
       * apply interp_lam_rr. exact fA. exact ft.
-      * apply piTy_HO_typing.
-        ** intros γ Hγ. refine (transpS (fun X => iA γ ∈ X) _ (vA γ Hγ)). now apply el_univTy.
-        ** intros γa Hγa. apply (vB γa Hγa).
-      * unfold ru. apply lamTm_HO_typing.
-        ** intros γ Hγ. refine (transpS (fun X => iA γ ∈ X) _ (vA γ Hγ)). now apply el_univTy.
-        ** intros γa Hγa. apply (vB γa Hγa).
-        ** intros γa Hγa. apply (vt γa Hγa).
+      * apply piTy_HO_typing. exact vA. exact vB. 
+      * unfold ru. apply lamTm_HO_typing. exact vA. exact vB. exact vt. 
     (* lambda (irrelevant relevant) *)
-    + econstructor.
+    + destruct (functional_ctx Γ fΓ H1) ; clear H1. destruct (functional_tm A fA H3) ; clear H3. econstructor.
       * exact fΓ.
       * apply interp_pi_ir. exact fA. exact fB.
       * apply interp_lam_ir. exact fA. exact ft.
-      * apply piTy_HO_typing_ir.
-        ** intros γ Hγ. refine (transpS (fun X => iA γ ∈ X) _ (vA γ Hγ)). now apply el_propTy.
-        ** intros γa Hγa. apply (vB γa Hγa).
-      * unfold ru. apply lamTm_HO_typing_ir.
-        ** intros γ Hγ. refine (transpS (fun X => iA γ ∈ X) _ (vA γ Hγ)). now apply el_propTy.
-        ** intros γa Hγa. apply (vB γa Hγa).
-        ** intros γa Hγa. apply (vt γa Hγa).
-  - destruct mt as [ iΓ' fΓ' iB fB vB vt ]. inversion fΓ' ; subst ; clear fΓ'.
-    all: destruct (functional_ctx Γ fΓ H3) ; clear H3. 
-    all: destruct (functional_tm A fA H4) ; clear H4. 
-    all: inversion fS ; subst ; clear fS.
+      * apply piTy_HO_typing_ir. exact vA. exact vB.
+      * unfold ru. apply lamTm_HO_typing_ir. exact vA. exact vB. exact vt.
+  - destruct mt as [ iΓ' fΓ' iB fB vB vt ]. destruct i as [ i | ] ; destruct mA as [ iΓ fΓ iA fA vA ].
+    all: inversion fΓ' ; subst ; clear fΓ'.
     (* lambda (relevant irrelevant) *)
-    + econstructor.
+    + destruct (functional_ctx Γ fΓ H3) ; clear H3. destruct (functional_tm A fA H4) ; clear H4. econstructor.
       * exact fΓ.
       * apply interp_pi_ri. exact fA. exact fB.
-      * apply forallTy_HO_typing.
-        ** intros γ Hγ. refine (transpS (fun X => iA γ ∈ X) _ (vA γ Hγ)). now apply el_univTy.
-        ** intros γa Hγa. apply (vB γa Hγa).
-      * apply ilamTm_HO_typing.
-        ** intros γ Hγ. refine (transpS (fun X => iA γ ∈ X) _ (vA γ Hγ)). now apply el_univTy.
-        ** intros γa Hγa. apply (vB γa Hγa).
-        ** intros γa Hγa. apply (vt γa Hγa).
+      * apply forallTy_HO_typing. exact vA. exact vB.
+      * apply ilamTm_HO_typing. exact vA. exact vB. exact vt.
     (* lambda (irrelevant irrelevant) *)
-    + econstructor.
+    + destruct (functional_ctx Γ fΓ H1) ; clear H1. destruct (functional_tm A fA H3) ; clear H3. econstructor. 
       * exact fΓ.
       * apply interp_pi_ii. exact fA. exact fB.
-      * apply forallTy_HO_typing.
-        ** apply boxTy_HO_typing. intros γ Hγ. refine (transpS (fun X => iA γ ∈ X) _ (vA γ Hγ)). now apply el_propTy.
-        ** intros γa Hγa. apply (vB γa Hγa).
+      * apply forallTy_HO_typing. 
+        ** apply boxTy_HO_typing. exact vA. 
+        ** exact vB.
       * apply ilamTm_HO_typing.
-        ** apply boxTy_HO_typing. intros γ Hγ. refine (transpS (fun X => iA γ ∈ X) _ (vA γ Hγ)). now apply el_propTy.
-        ** intros γa Hγa. apply (vB γa Hγa).
-        ** intros γa Hγa. apply (vt γa Hγa).
+        ** apply boxTy_HO_typing. exact vA.
+        ** exact vB.
+        ** exact vt.
 Qed.
 
 Lemma model_app (Γ : ctx) (i j : level) (A B t u : term) (tA : Γ ⊢< Ax i > A : Sort i) (mA : model_typing Γ (Ax i) A (Sort i))
